Tests/Tactics/ReduceFetchInst.lean
@@ -20,3 +20,19 @@ example (h : s.program = sha512_program_map) :
 example (h : s.program = sha512_program_map) :
     fetch_inst 0x126c98#64 s = (some 0xf84107fd#32) := by
   simp (config := {ground := false}) only [reduceFetchInst]
+
+/-! ## Tests for `refuceDecodeInst` simproc -/
+
+/--
+error: unsolved goals
+z : Option ArmInst
+⊢ some
+      (ArmInst.LDST
+        (LDSTInst.Advanced_simd_multiple_struct
+          { _fixed1 := 0#1, Q := 1#1, _fixed2 := 24#7, L := 1#1, _fixed3 := 0#6, opcode := 7#4, size := 3#2, Rn := 0#5,
+            Rt := 17#5 })) =
+    z
+-/
+#guard_msgs in
+example : decode_raw_inst 1279294481#32 = z := by
+  simp (config := {ground := false}) only [reduceDecodeInst]
